DenotationalLean.lean
@@ -2,5 +2,6 @@
 -- Import modules here that should be built as part of the library.
 import DenotationalLean.ADeriv
 import DenotationalLean.BDeriv
+import DenotationalLean.CDeriv
 import DenotationalLean.Imp
 import DenotationalLean.State
